prove transitivity of PDA.reaches

autth/test.lean
@@ -7,66 +7,6 @@ import Mathlib.Computability.ContextFreeGrammar
 
 import Mathlib.Computability.EpsilonNFA
 
-structure PDA  (Q: Type)(T: Type)(S: Type) where
-  initial_state : Q
-  start_symbol : S
-  final_states : Set Q
-  transition_fun : Q → T → S → Set (Q × List S)
-  transition_fun' : Q → S → Set (Q × List S)
-
-namespace PDA
-
-structure conf
-    {Q T S: Type} (p : PDA Q T S) where
-  state : Q
-  input : List T
-  stack : List S
-
-
-
-
-def step {Q T S : Type} {pda : PDA Q T S} (r₁ : conf pda) : Set (conf pda) :=
-  match r₁ with
-    | ⟨q,a::w,Z::α⟩ =>
-        {r₂ : conf pda | ∃ (p:Q) (β:List S), (p,β) ∈ pda.transition_fun q a Z ∧
-                          r₂=⟨p, w, (β ++ α)⟩ } ∪
-        {r₂ : conf pda | ∃(p:Q)(β:List S), (p,β) ∈ pda.transition_fun' q Z ∧
-                          r₂=⟨p, a :: w, (β ++ α)⟩}
-    | ⟨q,Nil,Z::α⟩ => {r₂ : conf pda | ∃(p:Q)(β:List S), (p,β) ∈ pda.transition_fun' q Z ∧
-                                         r₂=⟨p, Nil, (β ++ α)⟩}
-    | ⟨q,w,Nil⟩ => {r₂ : conf pda | r₂ = ⟨q,w,Nil⟩} -- Empty stack
-
-def stepSet {Q T S : Type} {pda : PDA Q T S} (R : Set (conf pda)) : Set (conf pda) :=
-  ⋃ r ∈ R , step r
-
-def stepSetN {Q T S : Type} {pda : PDA Q T S} (n : ℕ) (R : Set (conf pda))  : Set (conf pda) :=
-  match n with
-  | 0 => R
-  | Nat.succ m => stepSet (stepSetN m R)
-
-
-/-def stepRel {Q T S : Type} {pda : PDA Q T S} (r₁ : PDA_id pda)(r₂ : PDA_id pda) : Prop :=
-  r₂ ∈ step r₁-/
-
-inductive reaches' {Q T S : Type} {pda : PDA Q T S}  : conf pda→ conf pda→Prop :=
-  | base : (r₁ : conf pda) → reaches' r₁ r₁
-  | step : {r₁ r' r₂ : conf pda} → (r'∈ step r₁) → (reaches' r' r₂) → reaches' r₁ r₂
-
-def reachesN {Q T S : Type} {pda : PDA Q T S} (n : ℕ) (r₁ : conf pda)(r₂ : conf pda) : Prop :=
-  r₂ ∈ stepSetN n {r₁}
-
-def reaches {Q T S : Type} {pda : PDA Q T S}  (r₁ : conf pda)(r₂ : conf pda) : Prop :=
-  ∃n:ℕ, r₂ ∈ stepSetN n {r₁}
-
-
-def acceptsByEmptyStack {Q T S : Type} (pda : PDA Q T S) : Language T :=
-  {w : List T | ∃q:Q, reaches (⟨pda.initial_state, w, [pda.start_symbol]⟩ : conf pda) ⟨q,[],[]⟩ }
-
-def acceptsByFinalState {Q T S : Type} (pda : PDA Q T S) : Language T :=
-  {w : List T | ∃q ∈ pda.final_states,∃ γ:List S,
-      reaches (⟨pda.initial_state, w, [pda.start_symbol]⟩ : conf pda) ⟨q,[],γ⟩ }
-
-
 inductive alph where
   | a
   | b
