autth/PDA.lean
@@ -1,0 +1,109 @@
+import Mathlib.Data.Set.Lattice
+import Mathlib.Data.Set.Function
+import Mathlib.Tactic
+import Mathlib.Data.List.Join
+import Mathlib.Util.Delaborators
+import Mathlib.Computability.ContextFreeGrammar
+
+import Mathlib.Computability.EpsilonNFA
+
+structure PDA  (Q: Type)(T: Type)(S: Type) where
+  initial_state : Q
+  start_symbol : S
+  final_states : Set Q
+  transition_fun : Q → T → S → Set (Q × List S)
+  transition_fun' : Q → S → Set (Q × List S)
+
+namespace PDA
+
+@[ext]
+structure conf
+    {Q T S: Type} (p : PDA Q T S) where
+  state : Q
+  input : List T
+  stack : List S
+
+def step {Q T S : Type} {pda : PDA Q T S} (r₁ : conf pda) : Set (conf pda) :=
+  match r₁ with
+    | ⟨q,a::w,Z::α⟩ =>
+        {r₂ : conf pda | ∃ (p:Q) (β:List S), (p,β) ∈ pda.transition_fun q a Z ∧
+                          r₂=⟨p, w, (β ++ α)⟩ } ∪
+        {r₂ : conf pda | ∃(p:Q)(β:List S), (p,β) ∈ pda.transition_fun' q Z ∧
+                          r₂=⟨p, a :: w, (β ++ α)⟩}
+    | ⟨q,Nil,Z::α⟩ => {r₂ : conf pda | ∃(p:Q)(β:List S), (p,β) ∈ pda.transition_fun' q Z ∧
+                                         r₂=⟨p, Nil, (β ++ α)⟩}
+    | ⟨q,w,Nil⟩ => {r₂ : conf pda | r₂ = ⟨q,w,Nil⟩} -- Empty stack
+
+def stepSet {Q T S : Type} {pda : PDA Q T S} (R : Set (conf pda)) : Set (conf pda) :=
+  ⋃ r ∈ R , step r
+
+def stepSetN {Q T S : Type} {pda : PDA Q T S} (n : ℕ) (R : Set (conf pda))  : Set (conf pda) :=
+  match n with
+  | 0 => R
+  | Nat.succ m => stepSet (stepSetN m R)
+
+
+/-def stepRel {Q T S : Type} {pda : PDA Q T S} (r₁ : PDA_id pda)(r₂ : PDA_id pda) : Prop :=
+  r₂ ∈ step r₁-/
+
+inductive reaches' {Q T S : Type} {pda : PDA Q T S}  : conf pda→ conf pda→Prop :=
+  | base : (r₁ : conf pda) → reaches' r₁ r₁
+  | step : {r₁ r' r₂ : conf pda} → (r'∈ step r₁) → (reaches' r' r₂) → reaches' r₁ r₂
+
+def reachesN {Q T S : Type} {pda : PDA Q T S} (n : ℕ) (r₁ : conf pda)(r₂ : conf pda) : Prop :=
+  r₂ ∈ stepSetN n {r₁}
+
+def reaches {Q T S : Type} {pda : PDA Q T S}  (r₁ : conf pda)(r₂ : conf pda) : Prop :=
+  ∃n:ℕ, r₂ ∈ stepSetN n {r₁}
+
+
+def acceptsByEmptyStack {Q T S : Type} (pda : PDA Q T S) : Language T :=
+  {w : List T | ∃q:Q, reaches (⟨pda.initial_state, w, [pda.start_symbol]⟩ : conf pda) ⟨q,[],[]⟩ }
+
+def acceptsByFinalState {Q T S : Type} (pda : PDA Q T S) : Language T :=
+  {w : List T | ∃q ∈ pda.final_states,∃ γ:List S,
+      reaches (⟨pda.initial_state, w, [pda.start_symbol]⟩ : conf pda) ⟨q,[],γ⟩ }
+
+variable {Q T S : Type} {pda : PDA Q T S}
+
+theorem reaches_refl (r₁ : conf pda) : reaches r₁ r₁ := by
+  use 0; simp [stepSetN];
+
+theorem reachesN_of_add_one  {r₁ : conf pda}{r₂ : conf pda}{r₃ : conf pda}{n : ℕ}
+        (h₁:reachesN n r₁ r₂)(h₂:reachesN 1 r₂ r₃): reachesN (n+1) r₁ r₃ := by
+  simp [reachesN, stepSetN, stepSet] at *
+  use r₂
+
+theorem reachesN_trans  {r₁ : conf pda}{r₂ : conf pda}{r₃ : conf pda}{n m : ℕ}
+        (h₁:reachesN n r₁ r₂)(h₂:reachesN m r₂ r₃):∃k≤n+m, reachesN (k) r₁ r₃ := by
+  induction' m with m ih generalizing r₃
+  · simp [reachesN,stepSetN] at h₂
+    rw [←h₂] at h₁
+    use n
+    refine ⟨?_, h₁⟩
+    linarith
+  · rw [reachesN,stepSetN,stepSet] at h₂
+    simp at h₂
+    obtain ⟨c,h⟩ :=  h₂
+    have r₂_reaches_c: reachesN m r₂ c := by
+      simp [reachesN, stepSetN, stepSet] at *
+      exact h.1
+    apply ih at r₂_reaches_c
+    have c_reaches_r₃ : reachesN 1 c r₃ := by
+      simp [reachesN, stepSetN, stepSet] at *
+      exact h.2
+    obtain ⟨k,h⟩ := r₂_reaches_c
+    use k+1
+    constructor
+    linarith
+    exact reachesN_of_add_one h.2 c_reaches_r₃
+
+theorem reaches_trans  {r₁ : conf pda}{r₂ : conf pda}{r₃ : conf pda}
+        (h₁:reaches r₁ r₂)(h₂:reaches r₂ r₃): reaches r₁ r₃ := by
+  rw [reaches] at *
+  obtain ⟨n,h⟩ := h₁
+  obtain ⟨m,h'⟩ := h₂
+  rw [←reachesN] at *
+  rcases reachesN_trans h h' with ⟨k,h⟩
+  use k
+  exact h.2
